# Root Function Recurrence Relations

These recurrence relations are of the form:

T(n) = T(âˆšn) + f(n)


Or more generally:

T(n) = T(n^r) + f(n), where 0 < r < 1

They occur in certain **recursive algorithms** where the input size is reduced drastically â€” not by a constant factor (like n/2), but by taking a **root** of the input.

---

## Key Idea

Letâ€™s analyze how many times we can apply `âˆš` to `n` until it reduces to a constant:

### Example:
If `T(n) = T(âˆšn) + 1`, how many times can you apply `âˆš` until `n = 2`?

Letâ€™s define:

n â†’ âˆšn â†’ â´âˆšn â†’ ... â†’ log log n steps


So the **depth of recursion** is `O(log log n)`, and work at each level is constant (`+1`), so:

T(n) = O(log log n)


---

## ðŸ“š Common Root-Based Recurrences

| Recurrence                    | Time Complexity      | Reasoning                       |
|------------------------------|----------------------|----------------------------------|
| T(n) = T(âˆšn) + 1             | O(log log n)         | Each step halves the log        |
| T(n) = T(âˆšn) + log n         | O(log n)             | Sum of logs                     |
| T(n) = T(âˆšn) + âˆšn            | O(âˆšn)                | Decreases faster than linear    |
| T(n) = T(n^1/3) + n          | O(n)                 | Shrinks even faster than âˆšn     |

---

## Technique: Change of Variables

To solve `T(n) = T(âˆšn) + f(n)`, do a change of variables:

Let `n = 2^k` â†’ `logâ‚‚(n) = k`  

So, `âˆšn = 2^{k/2}`

Now rewrite:

T(2^k) = T(2^{k/2}) + f(2^k)

Let S(k) = T(2^k)

Then: S(k) = S(k/2) + f(2^k)


Now solve `S(k)` with standard methods (recursion tree or Master Theorem), then convert back to `n`.

---

## Summary Table

| Original Recurrence           | Substitution Form              | Final Complexity      |
|------------------------------|--------------------------------|-----------------------|
| T(n) = T(âˆšn) + 1             | S(k) = S(k/2) + 1              | O(log log n)          |
| T(n) = T(âˆšn) + log n         | S(k) = S(k/2) + k              | O(log n)              |
| T(n) = T(âˆšn) + âˆšn            | Complex, use summation         | O(âˆšn)                 |

---

## References

- Abdul Bariâ€™s Recurrence Relation Lectures


